$$
y' = f(x)g(y)
$$

$$
x^2y^2y'+1 = y
$$

$$
x^2y^2\dfrac{dy}{dx} = y - 1
$$

$$
x^2(y-1)\,dx
$$

$$
x^2y^2\,dy = (y-1)\,dx
$$

$$
y' = 3\sqrt[3]{y^2}; y(2) = 0
$$

$$
y'\ctg{x}+y = 2; y(x) \to -1, при\,x \to 0
$$

$$
xy\,dx + (x+1)\,dy = 0
$$

$$
\begin{cases}
\dot{x} = y + 2e^t\\
\dot{y} = x + t^2
\end{cases}
$$


$$
\begin{cases}
\dot{x} = y - 5\cos{t}\\
\dot{y} = 2x + y
\end{cases}
$$



$$
\dot{x} = Ax, A = \begin{pmatrix}
3&0\\
0&3
\end{pmatrix}
$$

$$
\dot{x} = Ax, A = \begin{pmatrix}
1&1\\
2&0
\end{pmatrix}
$$